Prove lemmas towards `TreeAutomaton.reachable_preserves_confluence`

Eqsat/TreeAutomaton/Reachable.lean
@@ -1,8 +1,8 @@
 import Eqsat.TreeAutomaton.Basic
 
-namespace TreeAutomaton
-
 variable [Signature S] {auto : TreeAutomaton S Q}
+
+namespace TreeAutomaton
 
 -- A given state is reachable (from a ground term) if it is the destination of a transition where
 -- all source states are reachable. Note that this condition is vacuously satisfied for constants.
@@ -13,17 +13,17 @@ inductive IsReachableState (auto : TreeAutomaton S Q) : Q → Prop where
 abbrev ReachableState (auto : TreeAutomaton S Q) : Type :=
   { q // auto.IsReachableState q }
 
-def IsReachableTransition (auto : TreeAutomaton S Q) (tr : Transition S Q) : Prop :=
-  ∀ i, auto.IsReachableState <| tr.srcs i
-
-def Transition.liftReachable {auto : TreeAutomaton S Q} (tr : Transition S auto.ReachableState) :
+def Transition.expand {auto : TreeAutomaton S Q} (tr : Transition S auto.ReachableState) :
     Transition S Q where
   sym  := tr.sym
   srcs := (tr.srcs ·)
   dst  := tr.dst
 
+def IsReachableTransition (auto : TreeAutomaton S Q) (tr : Transition S Q) : Prop :=
+  ∀ i, auto.IsReachableState <| tr.srcs i
+
 def reachableTrans (auto : TreeAutomaton S Q) : Set (Transition S auto.ReachableState) :=
-  { tr | auto.IsReachableTransition tr.liftReachable }
+  { tr | tr.expand ∈ auto.trans ∧ auto.IsReachableTransition tr.expand }
 
 def reachableFinal (auto : TreeAutomaton S Q) : Set auto.ReachableState :=
   { q | ↑q ∈ auto.final ∧ auto.IsReachableState q }
@@ -33,7 +33,140 @@ def reachable (auto : TreeAutomaton S Q) : TreeAutomaton S auto.ReachableState w
   trans := auto.reachableTrans
   final := auto.reachableFinal
 
-def reachable_preserves_confluence {auto : TreeAutomaton S Q} (con : auto.trs.Confluent) :
+end TreeAutomaton
+
+section Expand
+
+@[simp]
+def Pattern.expand : Pattern (S ⨄ auto.ReachableState) V → Pattern (S ⨄ Q) V
+  | (v : V)        => v
+  | (.sig fn) ° as => fn ° (expand <| as ·)
+  | (.ext fn) ° as => fn ° (expand <| as ·)
+
+theorem Pattern.expand_inj {p₁ p₂ : Pattern (S ⨄ auto.ReachableState) V}
+    (h : p₁.expand = p₂.expand) : p₁ = p₂ := by
+  induction p₁ generalizing p₂ <;> cases p₂
+  case var.var => simp_all [expand]
+  case var.app fn _ => cases fn <;> contradiction
+  case app.var fn₁ _ _ _ => cases fn₁ <;> contradiction
+  case app.app fn₁ _ ih fn₂ _ =>
+    cases fn₁ <;> cases fn₂
+    case sig.ext => injections
+    case ext.sig => injections
+    case sig.sig =>
+      injections; subst_vars
+      congr
+      ext i
+      have h := congr (eq_of_heq ‹_›) (rfl : i = i)
+      exact ih _ h
+    case ext.ext =>
+      injections
+      congr
+      next h => exact Subtype.val_inj.mp h
+      next h _ =>
+        ext i
+        have h := congr h (rfl : i = i)
+        exact ih _ h
+
+@[simp]
+def Pattern.expand_vars (p : Pattern (S ⨄ auto.ReachableState) V) : p.expand.vars = p.vars := by
+  induction p
+  case var => rfl
+  case app fn _ ih => cases fn <;> simp [ih]
+
+@[simp]
+def Rewrite.expand (rw : Rewrite (S ⨄ auto.ReachableState) V) : Rewrite (S ⨄ Q) V where
+  lhs := rw.lhs.expand
+  rhs := rw.rhs.expand
+  sub := by simp [rw.sub]
+
+def Subst.expand (σ : Subst (S ⨄ auto.ReachableState) V) : Subst (S ⨄ Q) V :=
+  fun i => (σ i).expand
+
+theorem TreeAutomaton.mem_reachable_trans (mem : tr ∈ auto.reachable.trans) :
+    tr.expand ∈ auto.trans := by
+  simp_all [reachable, reachableTrans]
+
+theorem TreeAutomaton.mem_reachable_trs (mem : rw ∈ auto.reachable.trs) : rw.expand ∈ auto.trs := by
+  have ⟨tr, h₁, h₂⟩ := mem_trs_to_trans mem
+  rw [Transition.toRewrite] at h₂
+  simp only [trs, Rewrite.expand, Set.mem_image, ← h₂, Pattern.expand]
+  exists tr.expand, mem_reachable_trans h₁
+  simp [Transition.toRewrite]
+  refine ⟨⟨rfl, ?_⟩, rfl, funext (·.elim0)⟩
+  ext i; congr; ext i; exact i.elim0
+
+theorem Args.set_expand (as : Term.Args fn) (a : Term <| S ⨄ auto.ReachableState) :
+    (as[↑i := a] · |>.expand) = (as · |>.expand)[i := a.expand] := by
+  ext i; cases fn
+  all_goals simp only [set]; split <;> rfl
+
+theorem TRS.Step.expand (s : t₁ -[auto.reachable]→ t₂) : t₁.expand -[auto]→ t₂.expand := by
+  induction s
+  case subst σ mem =>
+    have := Step.subst σ.expand <| TreeAutomaton.mem_reachable_trs mem
+    simp_all
+  case child a fn as i s ih =>
+    cases fn
+    all_goals
+      rename_i fn
+      simp only [Pattern.expand]
+      erw [Args.set_expand as a]
+      exact Step.child (a := a.expand) fn (as · |>.expand) ih
+
+open TreeAutomaton in
+theorem TRS.Step.restrict {t₁ : Term (S ⨄ auto.ReachableState)} (s : t₁.expand -[auto]→ t₂) :
+    ∃ r : Term (S ⨄ auto.ReachableState), (t₂ = r.expand) ∧ t₁ -[auto.reachable]→ r := by
+  generalize hl : t₁.expand = lhs at s
+  induction s generalizing t₁
+  case subst mem =>
+    simp at *
+    have ⟨tr, _, ht⟩ := mem_trs_to_trans mem
+    rw [Transition.toRewrite] at ht
+    have hd : auto.IsReachableState tr.dst := sorry
+    exists (⟨tr.dst, hd⟩ : auto.ReachableState)
+    simp only [← ht] at ⊢ hl
+    constructor
+    · congr; ext i; exact i.elim0
+    · have ⟨trr, ht₁, ht₂⟩ : ∃ trr : Transition S auto.ReachableState, trr.expand = tr ∧ trr ∈ auto.reachable.trans :=
+        sorry -- It might suffice to prove just ht₁ and then deduce ht₂ from left✝
+      subst ht₁
+      have := step_of_transition ht₂
+      -- bubble up the expand throught hl, then rewrite in the goal, the rest should follow
+      sorry
+  case child a fn as i s ih =>
+    let fn₁ ° as₁ := t₁
+    cases fn₁
+    all_goals
+      rw [Pattern.expand] at hl
+      injection hl with hl₁ hl₂
+      subst hl₁ hl₂
+      have ⟨r, hr, s'⟩ := ih rfl
+      subst hr
+      erw [← Args.set_expand as₁ r, ← Pattern.expand]
+      exact ⟨_, rfl, .child _ _ s'⟩
+
+theorem TRS.Steps.expand (s : t₁ -[auto.reachable]→* t₂) : t₁.expand -[auto]→* t₂.expand := by
+  induction s
+  case refl => rfl
+  case tail tl ih => exact tail ih tl.expand
+
+theorem TRS.Steps.restrict {t₁ : Term (S ⨄ auto.ReachableState)} (s : t₁.expand -[auto]→* t₂) :
+    ∃ r : Term (S ⨄ auto.ReachableState), (t₂ = r.expand) ∧ (t₁ -[auto.reachable]→* r) := by
+  induction s
+  case refl => exact ⟨_, rfl, .refl⟩
+  case tail tl ih =>
+    obtain ⟨_, hr, hd⟩ := ih
+    have ⟨_, hr, tl⟩ := (hr ▸ tl).restrict
+    exact ⟨_, hr, .tail hd tl⟩
+
+end Expand
+
+def TreeAutomaton.reachable_preserves_confluence (con : auto.trs.Confluent) :
     auto.reachable.trs.Confluent := by
   intro t t₁ t₂ s₁ s₂
-  sorry
+  have ⟨_, s₁, s₂⟩ := con s₁.expand s₂.expand
+  have ⟨r, hr₁, s₁⟩ := s₁.restrict
+  have ⟨_, hr₂, s₂⟩ := s₂.restrict
+  have hr := Pattern.expand_inj (hr₁ ▸ hr₂)
+  exact ⟨r, s₁, hr ▸ s₂⟩
